@prefix :        <http://purl.org/net/wicus-hwspecs#> .
@prefix dc:      <http://purl.org/dc/elements/1.1/> .
@prefix rdfs:    <http://www.w3.org/2000/01/rdf-schema#> .
@prefix owl2xml:  <http://www.w3.org/2006/12/owl2-xml#> .
@prefix terms:   <http://purl.org/dc/terms/> .
@prefix owl:     <http://www.w3.org/2002/07/owl#> .
@prefix xsd:     <http://www.w3.org/2001/XMLSchema#> .
@prefix rdf:     <http://www.w3.org/1999/02/22-rdf-syntax-ns#> .
@prefix vann:    <http://purl.org/vocab/vann/> .

terms:license
      a       owl:AnnotationProperty .

:unit
      a       owl:FunctionalProperty , owl:DatatypeProperty ;
      rdfs:comment "whw:unit defines the unit of measurement of a whw:Feature"^^rdfs:Literal ;
      rdfs:domain :Feature ;
      rdfs:range rdfs:Literal .

vann:preferredNamespaceUri
      a       owl:AnnotationProperty .

<http://purl.org/net/wicus-hwspecs>
      a       owl:Ontology ;
      dc:creator "http://delicias.dia.fi.upm.es/~isantana/"^^xsd:anyURI ;
      dc:title "The WICUS Hardware Specs ontology"@en ;
      terms:created "2013-06-14"^^xsd:date ;
      terms:description "The WICUS Hardware Specs ontology is describes the hardware characteristics of a computational infrastructure and the hardware requirements of a software component. This ontology is part of the WICUS Ontology network." ;
      terms:license "http://creativecommons.org/licenses/by-nc-sa/2.0/"^^xsd:anyURI ;
      terms:modified "2013-07-08"^^xsd:date ;
      vann:preferredNamespacePrefix
              "whw" ;
      vann:preferredNamespaceUri
              "http://purl.org/net/wicus-hwspecs#" ;
      owl:versionInfo "1.0" .

:hasHardwareComponent
      a       owl:ObjectProperty ;
      rdfs:comment "whw:hasHardwareComponent links a whw:HardwareSpec to the set of whw:HardwareComponent that compose it."^^rdfs:Literal ;
      rdfs:domain :HardwareSpec ;
      rdfs:range :HardwareComponent .

:HardwareSpec
      a       owl:Class ;
      rdfs:comment "A whw:HardwareSpec represents the set of hardware capabilities of a computational resource."^^rdfs:Literal .

:hasFeature
      a       owl:ObjectProperty ;
      rdfs:comment "whw:hasFeature links a whw:HardwareComponent to a whw:Feature defining its capabilities."^^rdfs:Literal ;
      rdfs:domain :HardwareComponent ;
      rdfs:range :Feature .

terms:created
      a       owl:AnnotationProperty .

dc:creator
      a       owl:AnnotationProperty .

:Network
      a       owl:Class ;
      rdfs:comment "A whw:Network is a specific type of whw:HardwareComponent representing the Network type of a computational resource."^^rdfs:Literal ;
      rdfs:subClassOf :HardwareComponent .

:Storage
      a       owl:Class ;
      rdfs:comment "A whw:Storage is a specific type of whw:HardwareComponent representing the storage capacity of a computational resource."^^rdfs:Literal ;
      rdfs:subClassOf :HardwareComponent .

vann:preferredNamespacePrefix
      a       owl:AnnotationProperty .

owl:Thing
      a       owl:Class .

:Feature
      a       owl:Class ;
      rdfs:comment "A whw:Feature represents a relevant characteristic of a component that define some of its capabilities."^^rdfs:Literal .

:HardwareComponent
      a       owl:Class ;
      rdfs:comment "A whw:HardwareComponent represents an element of the hardware stack of a computational resource."^^rdfs:Literal ;
      rdfs:subClassOf owl:Thing .

:Memory
      a       owl:Class ;
      rdfs:comment "A whw:Memory is a specific type of whw:HardwareComponent representing the RAM Memory of a computational resource."^^rdfs:Literal ;
      rdfs:subClassOf :HardwareComponent .

:value
      a       owl:FunctionalProperty , owl:DatatypeProperty ;
      rdfs:comment "whw:unit defines the value of a whw:Feature"^^rdfs:Literal ;
      rdfs:domain :Feature ;
      rdfs:range rdfs:Literal .

:CPU  a       owl:Class ;
      rdfs:comment "A whw:CPU is a specific type of whw:HardwareComponent representing the CPU of a computational resource."^^rdfs:Literal ;
      rdfs:subClassOf :HardwareComponent .

terms:modified
      a       owl:AnnotationProperty .

dc:title
      a       owl:AnnotationProperty .

terms:description
      a       owl:AnnotationProperty .
