@prefix dc:      <http://purl.org/dc/elements/1.1/> .
@prefix :        <http://purl.org/net/wicus#> .
@prefix wreq:    <http://purl.org/net/wicus-reqs#> .
@prefix terms:   <http://purl.org/dc/terms/> .
@prefix vann:    <http://purl.org/vocab/vann/> .
@prefix wsva:    <http://purl.org/net/wicus-sva#> .
@prefix whw:     <http://purl.org/net/wicus-hwspecs#> .
@prefix rdfs:    <http://www.w3.org/2000/01/rdf-schema#> .
@prefix owl2xml:  <http://www.w3.org/2006/12/owl2-xml#> .
@prefix wstack:  <http://purl.org/net/wicus-stack#> .
@prefix xsd:     <http://www.w3.org/2001/XMLSchema#> .
@prefix owl:     <http://www.w3.org/2002/07/owl#> .
@prefix rdf:     <http://www.w3.org/1999/02/22-rdf-syntax-ns#> .

:requiresHardware
      a       owl:ObjectProperty ;
      rdfs:comment "wicus:requiresHardware links a wstack:SoftwareComponent to a whw:HardwareSpec that defines the necessary hardware characteristics for deploying it."^^rdfs:Literal ;
      rdfs:domain wstack:SoftwareComponent ;
      rdfs:range whw:HardwareSpec .

terms:license
      a       owl:AnnotationProperty .

wreq:SoftwareRequirements
      a       owl:Class .

wsva:ImageAppliance
      a       owl:Class .

wstack:SoftwareStack
      a       owl:Class .

vann:preferredNamespaceUri
      a       owl:AnnotationProperty .

wreq:HardwareRequirements
      a       owl:Class .

wsva:ScientificVirtualAppliance
      a       owl:Class .

<http://purl.org/net/wicus>
      a       owl:Ontology ;
      dc:creator "http://delicias.dia.fi.upm.es/~isantana/"^^xsd:anyURI ;
      dc:title "The Workflow Infrastructure Conservation Using Semantics ontology" ;
      terms:created "2013-06-14"^^xsd:date ;
      terms:description """The WICUS ontology network is a set of ontologies designed to represent the information about the computational infrastructure involved on the execution of computational scientific experiments modelled as scientific workflows.
""" ;
      terms:license "http://creativecommons.org/licenses/by-nc-sa/2.0/"^^xsd:anyURI ;
      terms:modified "2013-07-08"^^xsd:date ;
      vann:preferredNamespacePrefix
              "wicus" ;
      vann:preferredNamespaceUri
              "http://purl.org/net/wicus#" ;
      owl:imports <http://purl.org/net/wicus-stack> , <http://purl.org/net/wicus-hwspecs> , <http://purl.org/net/wicus-reqs> , <http://purl.org/net/wicus-sva> ;
      owl:versionInfo "1.0" .

whw:HardwareSpec
      a       owl:Class .

terms:created
      a       owl:AnnotationProperty .

:composedBySoftwareStack
      a       owl:ObjectProperty ;
      rdfs:comment "wicus:composedBySoftwareStack links a wreq:SoftwareRequirements to a wstack:SoftwareStack defining the required software characteristics."^^rdfs:Literal ;
      rdfs:domain wreq:SoftwareRequirements ;
      rdfs:range wstack:SoftwareStack .

dc:creator
      a       owl:AnnotationProperty .

vann:preferredNamespacePrefix
      a       owl:AnnotationProperty .

:hasSoftwareStack
      a       owl:ObjectProperty ;
      rdfs:comment "wicus:hasSoftwareStack links a wsva:ScientificVirtualAppliance to a wstack:SoftwareStack defining the software characteristics of a scientific appliance."^^rdfs:Literal ;
      rdfs:domain wsva:ScientificVirtualAppliance ;
      rdfs:range wstack:SoftwareStack .

:hasHardwareSpecs
      a       owl:ObjectProperty ;
      rdfs:comment "wicus:hasHardwareSpecs links a wsva:ImageAppliance to a whw:HardwareSpec that defines the image hardware capabilities."^^rdfs:Literal ;
      rdfs:domain wsva:ImageAppliance ;
      rdfs:range whw:HardwareSpec .

:composedByHardwareSpec
      a       owl:ObjectProperty ;
      rdfs:comment "wicus:composedByHardwareSpec links a wreq:HardwareRequirements to a whw:HardwareSpec defining the required hardware characteristics."^^rdfs:Literal ;
      rdfs:domain wreq:HardwareRequirements ;
      rdfs:range whw:HardwareSpec .

terms:modified
      a       owl:AnnotationProperty .

dc:title
      a       owl:AnnotationProperty .

wstack:SoftwareComponent
      a       owl:Class .

terms:description
      a       owl:AnnotationProperty .
