@prefix :        <http://purl.org/net/wicus-sva#> .
@prefix dc:      <http://purl.org/dc/elements/1.1/> .
@prefix rdfs:    <http://www.w3.org/2000/01/rdf-schema#> .
@prefix owl2xml:  <http://www.w3.org/2006/12/owl2-xml#> .
@prefix terms:   <http://purl.org/dc/terms/> .
@prefix owl:     <http://www.w3.org/2002/07/owl#> .
@prefix xsd:     <http://www.w3.org/2001/XMLSchema#> .
@prefix rdf:     <http://www.w3.org/1999/02/22-rdf-syntax-ns#> .
@prefix vann:    <http://purl.org/vocab/vann/> .

:providedBy
      a       owl:ObjectProperty ;
      rdfs:comment "wsva:providedBy links a wsva:ImageAppliance to its corresponding wsva:InfrastructureProvider"^^rdfs:Literal ;
      rdfs:domain :ImageAppliance ;
      rdfs:range :InfrastructureProvider .

terms:license
      a       owl:AnnotationProperty .

:InfrastructureProvider
      a       owl:Class ;
      rdfs:comment "A wsva:InfrastructureProvider represents a service provider offering computational resources on demand."^^rdfs:Literal ;
      rdfs:subClassOf owl:Thing .

:ImageAppliance
      a       owl:Class ;
      rdfs:comment "A wsva:ImageAppliance represents an image specification supporting the instantiation of an appliance in an infrastructure provider platform."^^rdfs:Literal ;
      rdfs:subClassOf owl:Thing .

vann:preferredNamespaceUri
      a       owl:AnnotationProperty .

:ScientificVirtualAppliance
      a       owl:Class ;
      rdfs:comment "A wsva:ScientificVirtualAppliance represents a computational resource that may have been tuned for scientific purposes."^^rdfs:Literal .

:isSupportedBy
      a       owl:ObjectProperty ;
      rdfs:comment "wsva:isSupportedBy links a wsva:ScientificVirtualAppliance to the set of wsva:ImageAppliance that supports it."^^rdfs:Literal ;
      rdfs:domain :ScientificVirtualAppliance ;
      rdfs:range :ImageAppliance .

terms:created
      a       owl:AnnotationProperty .

<http://purl.org/net/wicus-sva>
      a       owl:Ontology ;
      dc:creator "http://delicias.dia.fi.upm.es/~isantana/"^^xsd:anyURI ;
      dc:title "The WICUS Scientific Virtual Appliance ontology"@en ;
      terms:created "2013-06-14"^^xsd:date ;
      terms:description "The WICUS Scientific Virtual Appliance ontology describes the virtual computational resources used for executing scientific experiments, usally as Virtual Machines deployed on a IaaS provider or a virtualization solution. This ontology is part of the WICUS Ontology network." ;
      terms:license "http://creativecommons.org/licenses/by-nc-sa/2.0/"^^xsd:anyURI ;
      terms:modified "2013-07-08"^^xsd:date ;
      vann:preferredNamespacePrefix
              "wsva" ;
      vann:preferredNamespaceUri
              "http://purl.org/net/wicus-sva#" ;
      owl:versionInfo "1.0" .

:VMImage
      a       owl:Class ;
      rdfs:comment "A wsva:VMImage represents a Virtual Machine image that defines the basis of an appliance."^^rdfs:Literal ;
      rdfs:subClassOf owl:Thing .

dc:creator
      a       owl:AnnotationProperty .

vann:preferredNamespacePrefix
      a       owl:AnnotationProperty .

:vmId
      a       owl:FunctionalProperty , owl:DatatypeProperty ;
      rdfs:comment "wsva:vmId defines the identifier of a wsva:VMImage"^^rdfs:Literal ;
      rdfs:domain :VMImage ;
      rdfs:range rdfs:Literal .

owl:Thing
      a       owl:Class .

:hasVMImage
      a       owl:FunctionalProperty , owl:ObjectProperty ;
      rdfs:comment "wsva:hasVMImage links a wsva:ImageAppliance to the set of wsva:VMImage that supports it."^^rdfs:Literal ;
      rdfs:domain :ImageAppliance ;
      rdfs:range :VMImage .

terms:modified
      a       owl:AnnotationProperty .

dc:title
      a       owl:AnnotationProperty .

terms:description
      a       owl:AnnotationProperty .
