@prefix :        <http://purl.org/net/wicus-reqs#> .
@prefix dc:      <http://purl.org/dc/elements/1.1/> .
@prefix rdfs:    <http://www.w3.org/2000/01/rdf-schema#> .
@prefix p-plan:  <http://purl.org/net/p-plan#> .
@prefix owl2xml:  <http://www.w3.org/2006/12/owl2-xml#> .
@prefix terms:   <http://purl.org/dc/terms/> .
@prefix owl:     <http://www.w3.org/2002/07/owl#> .
@prefix xsd:     <http://www.w3.org/2001/XMLSchema#> .
@prefix rdf:     <http://www.w3.org/1999/02/22-rdf-syntax-ns#> .
@prefix vann:    <http://purl.org/vocab/vann/> .

:SoftwareRequirements
      a       owl:Class ;
      rdfs:comment """A wreq:SoftwareRequirements is a specific type of wreq:ExecutionEnvironment, representing the software resources that must be provided to support the execution of a workflow.
"""^^rdfs:Literal ;
      rdfs:subClassOf :ExecutionEnvironment .

:AbstractWorkflow
      a       owl:Class ;
      rdfs:comment "A wreq:AbstractWorkflow is a specific type of wreq:Workflow in which at least one of its steps is not fully specified."^^rdfs:Literal ;
      rdfs:subClassOf :Workflow .

vann:preferredNamespaceUri
      a       owl:AnnotationProperty .

:HardwareRequirements
      a       owl:Class ;
      rdfs:comment """A wreq:HardwareRequirements is a specific type of wreq:ExecutionEnvironment, representing the hardware resources that must be provided to support the execution of a workflow.
"""^^rdfs:Literal ;
      rdfs:subClassOf :ExecutionEnvironment .

:Workflow
      a       owl:Class ;
      rdfs:comment "A wreq:Workflow is a specific type of p-plan:Plan, representing a computational scientific workflow from the point of view of its infrastructure."^^rdfs:Literal ;
      rdfs:subClassOf p-plan:Plan .

terms:requires
      a       owl:ObjectProperty .

:RequirementLevel
      a       owl:Class ;
      rdfs:comment "A wreq:RequirementLevel represents the degree of importance of a requirement."^^rdfs:Literal .

:ExecutionEnvironment
      a       owl:Class ;
      rdfs:comment "A wreq:ExecutionEnvironment represents the computational resources that must be provided to support the execution of a workflow."^^rdfs:Literal ;
      rdfs:subClassOf owl:Thing .

p-plan:isStepOfPlan
      a       owl:ObjectProperty .

:isStepOfWorkflow
      a       owl:ObjectProperty ;
      rdfs:comment "wreq:isStepOfWorkflow is a specific type of p-plan:isStepOfPlan that relates a wreq:WorkflowStep to the wreqs:Workflow that it belongs to."^^rdfs:Literal ;
      rdfs:domain :WorkflowStep ;
      rdfs:range :Workflow ;
      rdfs:subPropertyOf p-plan:isStepOfPlan .

terms:modified
      a       owl:AnnotationProperty .

p-plan:Step
      a       owl:Class .

dc:title
      a       owl:AnnotationProperty .

terms:license
      a       owl:AnnotationProperty .

p-plan:Plan
      a       owl:Class .

:WorkflowStep
      a       owl:Class ;
      rdfs:comment "A wreq:WorkflowStep is a specific type of p-plan:Step, representing a single step of a workflow."^^rdfs:Literal ;
      rdfs:subClassOf p-plan:Step .

<http://purl.org/net/wicus-reqs>
      a       owl:Ontology ;
      dc:creator "http://delicias.dia.fi.upm.es/~isantana/"^^xsd:anyURI ;
      dc:title "The WICUS Workflow Execution Requirements ontology"@en ;
      terms:created "2013-06-14"^^xsd:date ;
      terms:description "The WICUS Workflow Execution Requirements ontology relates a Scientific Workflow to the execution requirements and dependencies for executing it. This ontology is part of the WICUS Ontology network." ;
      terms:license "http://creativecommons.org/licenses/by-nc-sa/2.0/"^^xsd:anyURI ;
      terms:modified "2013-07-08"^^xsd:date ;
      vann:preferredNamespacePrefix
              "wreq" ;
      vann:preferredNamespaceUri
              "http://purl.org/net/wicus-reqs#" ;
      owl:versionInfo "1.0" .

:requires
      a       owl:ObjectProperty ;
      rdfs:comment "wreq:requires is a specific type of dcterms:requires that links a wreq:Worflow to the wreq:ExecutionEnvironment that must be available for executing it."^^rdfs:Literal ;
      rdfs:domain :Workflow ;
      rdfs:range :ExecutionEnvironment ;
      rdfs:subPropertyOf terms:requires .

terms:created
      a       owl:AnnotationProperty .

:hasLevel
      a       owl:ObjectProperty ;
      rdfs:comment "wreq:hasLevel links a wreq:ExecutionEnvironment to its corresponding wreq:RequirementLevel."^^rdfs:Literal ;
      rdfs:domain :ExecutionEnvironment ;
      rdfs:range :RequirementLevel .

dc:creator
      a       owl:AnnotationProperty .

vann:preferredNamespacePrefix
      a       owl:AnnotationProperty .

:hasConcreteWorkflow
      a       owl:ObjectProperty ;
      rdfs:comment "wreq:hasConcreteWorkflow links an wreq:AbstractWorkflow to the set of wreq:ConcreteWorkflow that implements it."^^rdfs:Literal ;
      rdfs:domain :AbstractWorkflow ;
      rdfs:range :ConcreteWorkflow .

owl:Thing
      a       owl:Class .

:ConcreteWorkflow
      a       owl:Class ;
      rdfs:comment "A wreq:ConcreteWorkflow is a specific type of wreq:Workflow in which all its steps are fully specified."^^rdfs:Literal ;
      rdfs:subClassOf :Workflow .

:hasSubworkflow
      a       owl:ObjectProperty ;
      rdfs:comment "wreq:hasSubworkflow links a wreq:Workflow to the subworkflows that compose it."^^rdfs:Literal ;
      rdfs:domain :Workflow ;
      rdfs:range :Workflow .

terms:description
      a       owl:AnnotationProperty .
